rules added in THoare, strong typing property proved in Determ

DetermA.v
@@ -1430,4 +1430,1717 @@ Lemma prmsTyping_aux4 (ftenv: funTC) (tenv: valTC)
 Defined.  
 
 
+(************************************************************************)
+
+
+Lemma ValueStrongTyping :
+  forall (v: Value) (t1: VTyp),   
+     ValueTyping v t1 -> 
+  forall t2: VTyp,  
+    ValueTyping v t2 -> 
+        t1 = t2.
+Proof.
+  intros.
+  inversion H; subst.
+  inversion H0; subst.
+  subst T T0.
+  rewrite H1 in H3.
+  assert (H2 = H4).
+  eapply loc_pi.
+  subst.
+  destruct t1.
+  destruct t2.
+  simpl in *.
+  revert H1.
+  revert H0.
+  revert v1.
+  rewrite <- H3.
+  intros.
+  assert (v0 = v1).
+  eapply loc_pi.
+  subst.
+  auto.
+Defined.  
+  
+Lemma IdStrongTyping :
+  forall (tenv: valTC) (x: Id) (t1: VTyp),   
+     IdTyping tenv x t1 -> 
+  forall t2: VTyp,  
+    IdTyping tenv x t2 -> 
+        t1 = t2.
+Proof.
+  intros.
+  inversion X; subst.
+  inversion X0; subst.
+  inversion X1; subst.
+  inversion X2; subst.
+  rewrite H in H0.
+  injection H0.
+  auto.
+Defined.  
+
+
+Lemma EnvStrongTyping :
+  forall (env: valEnv) (tenv1: valTC),   
+     EnvTyping env tenv1 -> 
+  forall tenv2: valTC,  
+    EnvTyping env tenv2 -> 
+        tenv1 = tenv2.
+Proof.
+  intros.
+  dependent induction env.
+  inversion X; subst.
+  inversion X0; subst.
+  auto.
+  inversion X; subst.
+  inversion X0; subst.
+  assert (ls2 = ls0).
+  eapply IHenv.
+  auto.
+  auto.
+  assert (v2 = v3).
+  eapply ValueStrongTyping.
+  eauto.
+  auto.
+  rewrite H.
+  rewrite H0.
+  auto.
+Defined.  
+  
+(*
+Lemma ListStrongTyping (ftenv: funTC) (tenv: valTC) (fenv: funEnv) :
+  forall (ls: list Exp) (ts1: list VTyp),   
+      Forall2T (ExpTyping ftenv tenv fenv) ls ts1 -> 
+  forall ts2: list VTyp,  
+      Forall2T (ExpTyping ftenv tenv fenv) ls ts2 -> 
+        ts1 = ts2.
+Proof.
+*)
+
+
+Definition UniEType :=
+  fun (ftenv: funTC) (tenv: valTC) (fenv: funEnv)
+      (e: Exp) (t1: VTyp) (k: ExpTyping ftenv tenv fenv e t1) => 
+  FEnvTyping fenv ftenv ->     
+  forall (t2: VTyp) (ftenv0: funTC),
+    FEnvTyping fenv ftenv0 ->       
+    ExpTyping ftenv0 tenv fenv e t2 -> 
+        t1 = t2.
+
+
+Definition UniPType :=
+  fun (ftenv: funTC) (tenv: valTC) (fenv: funEnv)
+      (ps: Prms) (pt1: PTyp) (k: PrmsTyping ftenv tenv fenv ps pt1) => 
+    FEnvTyping fenv ftenv ->
+    forall (pt2: PTyp) (ftenv0: funTC),
+      FEnvTyping fenv ftenv0 ->  
+      PrmsTyping ftenv0 tenv fenv ps pt2 -> 
+        pt1 = pt2.
+
+
+Definition UniQFType :=
+  fun (ftenv: funTC) (fenv: funEnv) 
+      (qf: QFun) (ft1: FTyp) (k: QFunTyping ftenv fenv qf ft1) => 
+    FEnvTyping fenv ftenv ->     
+    forall (ft2: FTyp) (ftenv0: funTC),
+    FEnvTyping fenv ftenv0 ->  
+      QFunTyping ftenv0 fenv qf ft2 -> 
+        ft1 = ft2.
+
+
+Definition UniETypeW (ftenv: funTC)
+                      (tenv: valTC) (fenv: funEnv)
+                      (e: Exp) (t1: VTyp) := 
+  ExpTyping ftenv tenv fenv e t1 ->  
+  FEnvTyping fenv ftenv ->     
+  forall (t2: VTyp) (ftenv0: funTC),
+    FEnvTyping fenv ftenv0 ->       
+    ExpTyping ftenv0 tenv fenv e t2 -> 
+        t1 = t2.
+
+
+Definition UniFTypeS :=
+  fun (f: Fun) (ft1: FTyp) (k: FunTyping f ft1) => 
+    forall (ft2: FTyp),  
+      FunTyping f ft2 -> 
+        ft1 = ft2.
+
+
+Definition UniFType :=
+  fun (f: Fun) (ft: FTyp) (k: FunTyping f ft) => 
+   (forall (fps: valTC) (t: VTyp),
+    ft = FT fps t ->      
+    forall (ftenv: funTC) (i: nat) (fenv: funEnv) 
+           (x: Id) (e0 e1: Exp),
+       FEnvTyping fenv ftenv ->      
+       f = FC fenv fps e0 e1 x i -> 
+       match i with 
+       | 0 => UniETypeW ftenv fps fenv e0 t
+       | S j => UniETypeW (updateE ftenv x ft) fps
+                (updateE fenv x (FC fenv fps e0 e1 x j)) e1 t 
+       end).
+
+
+
+Definition ExpTypingUni_rect :=
+  ExpTyping_str_rect UniFType UniQFType UniEType UniPType.
+
+
+Lemma ExpStrongTyping :
+  forall (ftenv: funTC) (tenv: valTC) (fenv: funEnv)
+         (e: Exp) (t1: VTyp),   
+      ExpTyping ftenv tenv fenv e t1 -> 
+      FEnvTyping fenv ftenv ->
+  forall (t2: VTyp) (ftenv0: funTC),
+    FEnvTyping fenv ftenv0 ->  
+    ExpTyping ftenv0 tenv fenv e t2 -> 
+        t1 = t2.
+Proof.
+eapply ExpTypingUni_rect.
+- (* SLL *)
+  unfold Par_SSL, UniEType.
+  intros.
+  constructor.
+- (* SLL *)
+  unfold Par_SSL, UniEType.
+  intros.
+  constructor.
+  assumption.
+  assumption.
+  assumption.
+- (* SSA *)  
+  unfold Par_SSA, UniFType.
+  constructor.
+- unfold Par_SSA, UniFType.
+  intros.
+  constructor.
+  assumption.
+  assumption.
+  assumption.
+- (* SSB *)
+  unfold Par_SSB, Par_SSA, UniFType.
+  intros.
+  econstructor.
+  exact m0.
+  exact m1.
+  assumption.
+  assumption.
+  assumption.
+  assumption.
+  assumption.
+  assumption.
+- (* Par_F *)
+  unfold UniFType, UniETypeW, UniEType.
+  intros.
+  inversion H0; subst.
+  inversion H1; subst. 
+  intros.
+  eapply H.
+  auto.
+  Focus 2.
+  eauto.
+  auto.
+- (* Par_F *)
+  unfold UniFType, UniETypeW, UniEType.
+  intros ftenv tenv fenv.
+  intros e0 e1 x n t.
+  intros K1 K2 K3 HP1 HP2.
+  intros fps t0 E3.
+  intros ftenv1 i fenv1 x0 e2 e3 K4 E4.
+  inversion E3; subst.
+  inversion E4; subst.
+  intros.
+  eapply HP1.
+  eapply updateFEnvLemma.
+  assumption.
+  assumption.
+  eassumption.
+  assumption.
+- (* Par_Q - QF *)
+  unfold UniQFType, UniFType, UniEType, UniETypeW.
+  intros.
+  inversion X1; subst.
+  destruct ft as [fps t].
+  specialize (H fps t eq_refl).
+  inversion k; subst.
+  + inversion X2; subst.
+    specialize (H ftenv1 0 fenv0 x e0 e1 X3 eq_refl).  
+    simpl in *.
+    assert (t = t0).
+    eapply H.
+    auto.
+    auto.
+    Focus 2.
+    eassumption.
+    auto.
+    rewrite H0.
+    auto.
+  + inversion X2; subst.
+    subst ftenv' fenv'.
+    subst ftenv'0 fenv'0. (* to compare X5 and X8 *)
+    specialize (H ftenv1
+                  (S n) fenv0 x e0 e1 X3 eq_refl).  
+    simpl in *.
+    assert (t = t0).
+    eapply H.
+    auto.
+    eapply updateFEnvLemma.
+    auto.
+    auto.
+    Focus 2.
+    eauto.
+    eapply updateFEnvLemma.
+    auto.
+    auto.
+    rewrite H0.
+    auto.
+
+- (* Par_Q - FVar *)  
+  unfold  UniQFType, UniFType, UniEType, UniETypeW, Par_SSB, Par_SSA.
+  intros.  
+  inversion X; subst.
+  clear X.
+  clear X3 X4.
+  destruct ft as [fps t].
+  specialize (H1 fps t eq_refl).  
+  inversion X2; subst.
+  destruct ft2.
+  destruct f.
+
+  inversion m; subst.
+  inversion X3; subst.
+  
+  +
+    inversion X; subst.
+    rewrite H0 in H4.
+    (*inversion X2; subst.
+    inversion X8; subst. *)
+    
+(***)    
+    assert (f0 = FC fenv fps e0 e1 x0 0).
+    eapply (envAppendCompare FunTyping ls0 ls8 ls1 ls3). 
+    eauto.
+    eauto.
+    eauto.
+    auto.
+    auto.
+        
+    rewrite H5 in *.
+  
+    specialize (H1 ftenv).  
+    specialize (H1 0 fenv x0 e0 e1). 
+    specialize (H1 X6 eq_refl).
+    simpl in *.
+    inversion X8; subst.
+
+    assert (t = ret_type).
+    eapply H1. 
+    auto.
+    auto.
+    Focus 2.
+    eauto.
+    auto.
+    rewrite H5.
+    auto.
+    
+  + inversion X; subst.
+    rewrite H0 in H4.
+    (* inversion X2; subst. 
+    inversion X9; subst. *)
+
+    assert (f0 = FC fenv fps e0 e1 x0 (S n0)).
+    eapply (envAppendCompare FunTyping ls0 ls8 ls1 ls3). 
+    eauto.
+    eauto.
+    eauto.
+    auto.
+    auto.
+
+    rewrite H5 in *.
+
+    specialize (H1 ftenv).  
+    specialize (H1 (S n0) fenv x0 e0 e1). 
+    specialize (H1 X6 eq_refl).
+    simpl in *.
+    inversion X9; subst.
+
+    assert (t = ret_type).
+    eapply H1. 
+    auto.
+    eapply updateFEnvLemma.
+    auto.
+    auto.
+    Focus 2.
+    eauto.
+    subst ftenv'0.
+    eapply updateFEnvLemma.
+    auto.
+    auto.
+    rewrite H5.
+    auto.
+    
+- (* modify *)
+  unfold UniEType.
+  intros ftenv tenv fenv T1 T2 VT1 VT2 XF q K H0 t ftenv0 H0' X.
+  inversion X; subst.
+  eapply inj_pair2 in H6.
+  eapply inj_pair2 in H6; subst.  
+  assert (VT4 = VT1).
+  eapply loc_pi.
+  subst.
+  assert (VT5 = VT2).
+  eapply loc_pi.
+  subst.
+  clear XF2.
+  reflexivity.
+  (* return *)
+- unfold UniEType.
+  intros.
+  inversion X1; subst.
+  inversion X2; subst.
+  inversion k; subst.
+  eapply ValueStrongTyping.
+  eauto.
+  eauto.
+  inversion k; subst.
+  eapply IdStrongTyping.
+  eauto.
+  auto.
+(* bindN *)
+- unfold UniEType.
+  intros.
+  inversion X1; subst.
+  eapply H0.
+  auto.
+  Focus 2.
+  eauto.
+  auto.
+(* bindS *)
+- unfold UniEType.
+  intros.
+  inversion X1; subst.
+  eapply H0.
+  auto.
+  Focus 2.
+  subst tenv'.
+  assert (t1 = t3).
+  eapply H.
+  auto.
+  Focus 2.
+  eauto.
+  auto.
+  rewrite H1.
+  eauto.
+  auto.
+- unfold UniEType.
+  intros.
+  inversion X1; subst.
+  eapply H.
+  eapply overrideEnvLemmaT.
+  assumption.
+  assumption.
+  Focus 2.
+  assert (tenvP = tenvP0).
+  eapply EnvStrongTyping.
+  eauto.
+  auto.
+  rewrite H0.
+  eauto.
+  eapply overrideEnvLemmaT.
+  auto.
+  auto.
+- unfold UniEType, UniQFType, UniPType.
+  intros.  
+  inversion X1; subst.
+  assert (FT fps t = FT fps0 t2).
+  eapply H.
+  auto.
+  eauto.
+  auto.
+  injection H1.
+  auto.
+- unfold UniEType.
+  intros.
+  inversion X1; subst.
+  eapply ValueStrongTyping.
+  eauto.
+  auto.
+- unfold UniEType.
+  intros.
+  inversion X1; subst.
+  eapply H0.
+  auto.
+  Focus 2.
+  eauto.
+  auto.
+- unfold UniEType, Par_SSL, UniPType.
+  intros.
+  dependent induction X; subst.
+  inversion X2; subst.
+  inversion X; subst.
+  auto.
+  destruct pt2.
+  destruct ts.
+  + inversion X2; subst.
+    inversion X3.
+  + inversion m; subst.
+    inversion X2; subst.
+    inversion X5; subst.
+    assert (PT bbs = PT ts).
+    {*  eapply IHX.
+      auto.
+      auto.
+      Focus 2.
+      econstructor.
+      eauto.
+      auto.
+   }   
+   injection H.
+   intro.
+   assert (b = v).
+   {* eapply p0.
+      auto.
+      Focus 2.
+      eauto.
+      auto.
+   }
+   rewrite H0.
+   rewrite H1.
+   auto.
+Qed.   
+
+
+
+Definition PrmsTypingUni_rect :=
+  PrmsTyping_str_rect UniFType UniQFType UniEType UniPType.
+
+
+Lemma PrmsStrongTyping :
+  forall (ftenv: funTC) (tenv: valTC) (fenv: funEnv)
+         (ps: Prms) (pt: PTyp)   
+         (k: PrmsTyping ftenv tenv fenv ps pt),  
+         UniPType ftenv tenv fenv ps pt k.
+Proof.
+eapply PrmsTypingUni_rect.
+- (* SLL *)
+  unfold Par_SSL, UniEType.
+  intros.
+  constructor.
+- (* SLL *)
+  unfold Par_SSL, UniEType.
+  intros.
+  constructor.
+  assumption.
+  assumption.
+  assumption.
+- (* SSA *)  
+  unfold Par_SSA, UniFType.
+  constructor.
+- unfold Par_SSA, UniFType.
+  intros.
+  constructor.
+  assumption.
+  assumption.
+  assumption.
+- (* SSB *)
+  unfold Par_SSB, Par_SSA, UniFType.
+  intros.
+  econstructor.
+  exact m0.
+  exact m1.
+  assumption.
+  assumption.
+  assumption.
+  assumption.
+  assumption.
+  assumption.
+- (* Par_F *)
+  unfold UniFType, UniETypeW, UniEType.
+  intros.
+  inversion H0; subst.
+  inversion H1; subst. 
+  intros.
+  eapply H.
+  auto.
+  Focus 2.
+  eauto.
+  auto.
+- (* Par_F *)
+  unfold UniFType, UniETypeW, UniEType.
+  intros ftenv tenv fenv.
+  intros e0 e1 x n t.
+  intros K1 K2 K3 HP1 HP2.
+  intros fps t0 E3.
+  intros ftenv1 i fenv1 x0 e2 e3 K4 E4.
+  inversion E3; subst.
+  inversion E4; subst.
+  intros.
+  eapply HP1.
+  eapply updateFEnvLemma.
+  assumption.
+  assumption.
+  eassumption.
+  assumption.
+- (* Par_Q - QF *)
+  unfold UniQFType, UniFType, UniEType, UniETypeW.
+  intros.
+  inversion X1; subst.
+  destruct ft as [fps t].
+  specialize (H fps t eq_refl).
+  inversion k; subst.
+  + inversion X2; subst.
+    specialize (H ftenv1 0 fenv0 x e0 e1 X3 eq_refl).  
+    simpl in *.
+    assert (t = t0).
+    eapply H.
+    auto.
+    auto.
+    Focus 2.
+    eassumption.
+    auto.
+    rewrite H0.
+    auto.
+  + inversion X2; subst.
+    subst ftenv' fenv'.
+    subst ftenv'0 fenv'0. (* to compare X5 and X8 *)
+    specialize (H ftenv1
+                  (S n) fenv0 x e0 e1 X3 eq_refl).  
+    simpl in *.
+    assert (t = t0).
+    eapply H.
+    auto.
+    eapply updateFEnvLemma.
+    auto.
+    auto.
+    Focus 2.
+    eauto.
+    eapply updateFEnvLemma.
+    auto.
+    auto.
+    rewrite H0.
+    auto.
+
+- (* Par_Q - FVar *)  
+  unfold  UniQFType, UniFType, UniEType, UniETypeW, Par_SSB, Par_SSA.
+  intros.  
+  inversion X; subst.
+  clear X.
+  clear X3 X4.
+  destruct ft as [fps t].
+  specialize (H1 fps t eq_refl).  
+  inversion X2; subst.
+  destruct ft2.
+  destruct f.
+
+  inversion m; subst.
+  inversion X3; subst.
+  
+  +
+    inversion X; subst.
+    rewrite H0 in H4.
+    (*inversion X2; subst.
+    inversion X8; subst. *)
+    
+(***)    
+    assert (f0 = FC fenv fps e0 e1 x0 0).
+    eapply (envAppendCompare FunTyping ls0 ls8 ls1 ls3). 
+    eauto.
+    eauto.
+    eauto.
+    auto.
+    auto.
+    
+    rewrite H5 in *.
+  
+    specialize (H1 ftenv).  
+    specialize (H1 0 fenv x0 e0 e1). 
+    specialize (H1 X6 eq_refl).
+    simpl in *.
+    inversion X8; subst.
+
+    assert (t = ret_type).
+    eapply H1. 
+    auto.
+    auto.
+    Focus 2.
+    eauto.
+    auto.
+    rewrite H5.
+    auto.
+    
+  + inversion X; subst.
+    rewrite H0 in H4.
+    (* inversion X2; subst. 
+    inversion X9; subst. *)
+
+    assert (f0 = FC fenv fps e0 e1 x0 (S n0)).
+    eapply (envAppendCompare FunTyping ls0 ls8 ls1 ls3). 
+    eauto.
+    eauto.
+    eauto.
+    auto.
+    auto.
+
+    rewrite H5 in *.
+
+    specialize (H1 ftenv).  
+    specialize (H1 (S n0) fenv x0 e0 e1). 
+    specialize (H1 X6 eq_refl).
+    simpl in *.
+    inversion X9; subst.
+
+    assert (t = ret_type).
+    eapply H1. 
+    auto.
+    eapply updateFEnvLemma.
+    auto.
+    auto.
+    Focus 2.
+    eauto.
+    subst ftenv'0.
+    eapply updateFEnvLemma.
+    auto.
+    auto.
+    rewrite H5.
+    auto.
+    
+- (* modify *)
+  unfold UniEType.
+  intros ftenv tenv fenv T1 T2 VT1 VT2 XF q K H0 t ftenv0 H0' X.
+  inversion X; subst.
+  eapply inj_pair2 in H6.
+  eapply inj_pair2 in H6; subst.  
+  assert (VT4 = VT1).
+  eapply loc_pi.
+  subst.
+  assert (VT5 = VT2).
+  eapply loc_pi.
+  subst.
+  clear XF2.
+  reflexivity.
+  (* return *)
+- unfold UniEType.
+  intros.
+  inversion X1; subst.
+  inversion X2; subst.
+  inversion k; subst.
+  eapply ValueStrongTyping.
+  eauto.
+  eauto.
+  inversion k; subst.
+  eapply IdStrongTyping.
+  eauto.
+  auto.
+(* bindN *)
+- unfold UniEType.
+  intros.
+  inversion X1; subst.
+  eapply H0.
+  auto.
+  Focus 2.
+  eauto.
+  auto.
+(* bindS *)
+- unfold UniEType.
+  intros.
+  inversion X1; subst.
+  eapply H0.
+  auto.
+  Focus 2.
+  subst tenv'.
+  assert (t1 = t3).
+  eapply H.
+  auto.
+  Focus 2.
+  eauto.
+  auto.
+  rewrite H1.
+  eauto.
+  auto.
+- unfold UniEType.
+  intros.
+  inversion X1; subst.
+  eapply H.
+  eapply overrideEnvLemmaT.
+  assumption.
+  assumption.
+  Focus 2.
+  assert (tenvP = tenvP0).
+  eapply EnvStrongTyping.
+  eauto.
+  auto.
+  rewrite H0.
+  eauto.
+  eapply overrideEnvLemmaT.
+  auto.
+  auto.
+- unfold UniEType, UniQFType, UniPType.
+  intros.  
+  inversion X1; subst.
+  assert (FT fps t = FT fps0 t2).
+  eapply H.
+  auto.
+  eauto.
+  auto.
+  injection H1.
+  auto.
+- unfold UniEType.
+  intros.
+  inversion X1; subst.
+  eapply ValueStrongTyping.
+  eauto.
+  auto.
+- unfold UniEType.
+  intros.
+  inversion X1; subst.
+  eapply H0.
+  auto.
+  Focus 2.
+  eauto.
+  auto.
+- unfold UniEType, Par_SSL, UniPType.
+  intros.
+  dependent induction X; subst.
+  inversion X2; subst.
+  inversion X; subst.
+  auto.
+  destruct pt2.
+  destruct ts.
+  + inversion X2; subst.
+    inversion X3.
+  + inversion m; subst.
+    inversion X2; subst.
+    inversion X5; subst.
+    assert (PT bbs = PT ts).
+    {*  eapply IHX.
+      auto.
+      auto.
+      Focus 2.
+      econstructor.
+      eauto.
+      auto.
+   }   
+   injection H.
+   intro.
+   assert (b = v).
+   {* eapply p0.
+      auto.
+      Focus 2.
+      eauto.
+      auto.
+   }
+   rewrite H0.
+   rewrite H1.
+   auto.
+Qed.   
+
+
+Definition QFunTypingUni_rect :=
+  QFunTyping_str_rect UniFType UniQFType UniEType UniPType.
+
+
+Lemma QFunStrongTyping :
+  forall (ftenv: funTC) (fenv: funEnv)
+         (qf: QFun) (ft: FTyp)  
+         (k: QFunTyping ftenv fenv qf ft), 
+     UniQFType ftenv fenv qf ft k.    
+Proof.
+eapply QFunTypingUni_rect.
+- (* SLL *)
+  unfold Par_SSL, UniEType.
+  intros.
+  constructor.
+- (* SLL *)
+  unfold Par_SSL, UniEType.
+  intros.
+  constructor.
+  assumption.
+  assumption.
+  assumption.
+- (* SSA *)  
+  unfold Par_SSA, UniFType.
+  constructor.
+- unfold Par_SSA, UniFType.
+  intros.
+  constructor.
+  assumption.
+  assumption.
+  assumption.
+- (* SSB *)
+  unfold Par_SSB, Par_SSA, UniFType.
+  intros.
+  econstructor.
+  exact m0.
+  exact m1.
+  assumption.
+  assumption.
+  assumption.
+  assumption.
+  assumption.
+  assumption.
+- (* Par_F *)
+  unfold UniFType, UniETypeW, UniEType.
+  intros.
+  inversion H0; subst.
+  inversion H1; subst. 
+  intros.
+  eapply H.
+  auto.
+  Focus 2.
+  eauto.
+  auto.
+- (* Par_F *)
+  unfold UniFType, UniETypeW, UniEType.
+  intros ftenv tenv fenv.
+  intros e0 e1 x n t.
+  intros K1 K2 K3 HP1 HP2.
+  intros fps t0 E3.
+  intros ftenv1 i fenv1 x0 e2 e3 K4 E4.
+  inversion E3; subst.
+  inversion E4; subst.
+  intros.
+  eapply HP1.
+  eapply updateFEnvLemma.
+  assumption.
+  assumption.
+  eassumption.
+  assumption.
+- (* Par_Q - QF *)
+  unfold UniQFType, UniFType, UniEType, UniETypeW.
+  intros.
+  inversion X1; subst.
+  destruct ft as [fps t].
+  specialize (H fps t eq_refl).
+  inversion k; subst.
+  + inversion X2; subst.
+    specialize (H ftenv1 0 fenv0 x e0 e1 X3 eq_refl).  
+    simpl in *.
+    assert (t = t0).
+    eapply H.
+    auto.
+    auto.
+    Focus 2.
+    eassumption.
+    auto.
+    rewrite H0.
+    auto.
+  + inversion X2; subst.
+    subst ftenv' fenv'.
+    subst ftenv'0 fenv'0. (* to compare X5 and X8 *)
+    specialize (H ftenv1
+                  (S n) fenv0 x e0 e1 X3 eq_refl).  
+    simpl in *.
+    assert (t = t0).
+    eapply H.
+    auto.
+    eapply updateFEnvLemma.
+    auto.
+    auto.
+    Focus 2.
+    eauto.
+    eapply updateFEnvLemma.
+    auto.
+    auto.
+    rewrite H0.
+    auto.
+
+- (* Par_Q - FVar *)  
+  unfold  UniQFType, UniFType, UniEType, UniETypeW, Par_SSB, Par_SSA.
+  intros.  
+  inversion X; subst.
+  clear X.
+  clear X3 X4.
+  destruct ft as [fps t].
+  specialize (H1 fps t eq_refl).  
+  inversion X2; subst.
+  destruct ft2.
+  destruct f.
+
+  inversion m; subst.
+  inversion X3; subst.
+  
+  +
+    inversion X; subst.
+    rewrite H0 in H4.
+    (*inversion X2; subst.
+    inversion X8; subst. *)
+    
+(***)    
+    assert (f0 = FC fenv fps e0 e1 x0 0).
+    eapply (envAppendCompare FunTyping ls0 ls8 ls1 ls3). 
+    eauto.
+    eauto.
+    eauto.
+    auto.
+    auto.
+    
+    rewrite H5 in *.
+  
+    specialize (H1 ftenv).  
+    specialize (H1 0 fenv x0 e0 e1). 
+    specialize (H1 X6 eq_refl).
+    simpl in *.
+    inversion X8; subst.
+
+    assert (t = ret_type).
+    eapply H1. 
+    auto.
+    auto.
+    Focus 2.
+    eauto.
+    auto.
+    rewrite H5.
+    auto.
+    
+  + inversion X; subst.
+    rewrite H0 in H4.
+    (* inversion X2; subst. 
+    inversion X9; subst. *)
+
+    assert (f0 = FC fenv fps e0 e1 x0 (S n0)).
+    eapply (envAppendCompare FunTyping ls0 ls8 ls1 ls3). 
+    eauto.
+    eauto.
+    eauto.
+    auto.
+    auto.
+    
+    rewrite H5 in *.
+
+    specialize (H1 ftenv).  
+    specialize (H1 (S n0) fenv x0 e0 e1). 
+    specialize (H1 X6 eq_refl).
+    simpl in *.
+    inversion X9; subst.
+
+    assert (t = ret_type).
+    eapply H1. 
+    auto.
+    eapply updateFEnvLemma.
+    auto.
+    auto.
+    Focus 2.
+    eauto.
+    subst ftenv'0.
+    eapply updateFEnvLemma.
+    auto.
+    auto.
+    rewrite H5.
+    auto.
+    
+- (* modify *)
+  unfold UniEType.
+  intros ftenv tenv fenv T1 T2 VT1 VT2 XF q K H0 t ftenv0 H0' X.
+  inversion X; subst.
+  eapply inj_pair2 in H6.
+  eapply inj_pair2 in H6; subst.  
+  assert (VT4 = VT1).
+  eapply loc_pi.
+  subst.
+  assert (VT5 = VT2).
+  eapply loc_pi.
+  subst.
+  clear XF2.
+  reflexivity.
+  (* return *)
+- unfold UniEType.
+  intros.
+  inversion X1; subst.
+  inversion X2; subst.
+  inversion k; subst.
+  eapply ValueStrongTyping.
+  eauto.
+  eauto.
+  inversion k; subst.
+  eapply IdStrongTyping.
+  eauto.
+  auto.
+(* bindN *)
+- unfold UniEType.
+  intros.
+  inversion X1; subst.
+  eapply H0.
+  auto.
+  Focus 2.
+  eauto.
+  auto.
+(* bindS *)
+- unfold UniEType.
+  intros.
+  inversion X1; subst.
+  eapply H0.
+  auto.
+  Focus 2.
+  subst tenv'.
+  assert (t1 = t3).
+  eapply H.
+  auto.
+  Focus 2.
+  eauto.
+  auto.
+  rewrite H1.
+  eauto.
+  auto.
+- unfold UniEType.
+  intros.
+  inversion X1; subst.
+  eapply H.
+  eapply overrideEnvLemmaT.
+  assumption.
+  assumption.
+  Focus 2.
+  assert (tenvP = tenvP0).
+  eapply EnvStrongTyping.
+  eauto.
+  auto.
+  rewrite H0.
+  eauto.
+  eapply overrideEnvLemmaT.
+  auto.
+  auto.
+- unfold UniEType, UniQFType, UniPType.
+  intros.  
+  inversion X1; subst.
+  assert (FT fps t = FT fps0 t2).
+  eapply H.
+  auto.
+  eauto.
+  auto.
+  injection H1.
+  auto.
+- unfold UniEType.
+  intros.
+  inversion X1; subst.
+  eapply ValueStrongTyping.
+  eauto.
+  auto.
+- unfold UniEType.
+  intros.
+  inversion X1; subst.
+  eapply H0.
+  auto.
+  Focus 2.
+  eauto.
+  auto.
+- unfold UniEType, Par_SSL, UniPType.
+  intros.
+  dependent induction X; subst.
+  inversion X2; subst.
+  inversion X; subst.
+  auto.
+  destruct pt2.
+  destruct ts.
+  + inversion X2; subst.
+    inversion X3.
+  + inversion m; subst.
+    inversion X2; subst.
+    inversion X5; subst.
+    assert (PT bbs = PT ts).
+    {*  eapply IHX.
+      auto.
+      auto.
+      Focus 2.
+      econstructor.
+      eauto.
+      auto.
+   }   
+   injection H.
+   intro.
+   assert (b = v).
+   {* eapply p0.
+      auto.
+      Focus 2.
+      eauto.
+      auto.
+   }
+   rewrite H0.
+   rewrite H1.
+   auto.
+Qed.   
+
+ 
+Definition FunTypingUni_rect :=
+  FunTyping_str_rect UniFType UniQFType UniEType UniPType.
+
+
+Lemma FunStrongTyping :
+  forall (f: Fun) (ft: FTyp) (k: FunTyping f ft),
+    UniFType f ft k.
+Proof.
+eapply FunTypingUni_rect.
+- (* SLL *)
+  unfold Par_SSL, UniEType.
+  intros.
+  constructor.
+- (* SLL *)
+  unfold Par_SSL, UniEType.
+  intros.
+  constructor.
+  assumption.
+  assumption.
+  assumption.
+- (* SSA *)  
+  unfold Par_SSA, UniFType.
+  constructor.
+- unfold Par_SSA, UniFType.
+  intros.
+  constructor.
+  assumption.
+  assumption.
+  assumption.
+- (* SSB *)
+  unfold Par_SSB, Par_SSA, UniFType.
+  intros.
+  econstructor.
+  exact m0.
+  exact m1.
+  assumption.
+  assumption.
+  assumption.
+  assumption.
+  assumption.
+  assumption.
+- (* Par_F *)
+  unfold UniFType, UniETypeW, UniEType.
+  intros.
+  inversion H0; subst.
+  inversion H1; subst. 
+  intros.
+  eapply H.
+  auto.
+  Focus 2.
+  eauto.
+  auto.
+- (* Par_F *)
+  unfold UniFType, UniETypeW, UniEType.
+  intros ftenv tenv fenv.
+  intros e0 e1 x n t.
+  intros K1 K2 K3 HP1 HP2.
+  intros fps t0 E3.
+  intros ftenv1 i fenv1 x0 e2 e3 K4 E4.
+  inversion E3; subst.
+  inversion E4; subst.
+  intros.
+  eapply HP1.
+  eapply updateFEnvLemma.
+  assumption.
+  assumption.
+  eassumption.
+  assumption.
+- (* Par_Q - QF *)
+  unfold UniQFType, UniFType, UniEType, UniETypeW.
+  intros.
+  inversion X1; subst.
+  destruct ft as [fps t].
+  specialize (H fps t eq_refl).
+  inversion k; subst.
+  + inversion X2; subst.
+    specialize (H ftenv1 0 fenv0 x e0 e1 X3 eq_refl).  
+    simpl in *.
+    assert (t = t0).
+    eapply H.
+    auto.
+    auto.
+    Focus 2.
+    eassumption.
+    auto.
+    rewrite H0.
+    auto.
+  + inversion X2; subst.
+    subst ftenv' fenv'.
+    subst ftenv'0 fenv'0. 
+    specialize (H ftenv1
+                  (S n) fenv0 x e0 e1 X3 eq_refl).  
+    simpl in *.
+    assert (t = t0).
+    eapply H.
+    auto.
+    eapply updateFEnvLemma.
+    auto.
+    auto.
+    Focus 2.
+    eauto.
+    eapply updateFEnvLemma.
+    auto.
+    auto.
+    rewrite H0.
+    auto.
+
+- (* Par_Q - FVar *)  
+  unfold  UniQFType, UniFType, UniEType, UniETypeW, Par_SSB, Par_SSA.
+  intros.  
+  inversion X; subst.
+  clear X.
+  clear X3 X4.
+  destruct ft as [fps t].
+  specialize (H1 fps t eq_refl).  
+  inversion X2; subst.
+  destruct ft2.
+  destruct f.
+
+  inversion m; subst.
+  inversion X3; subst.
+  
+  +
+    inversion X; subst.
+    rewrite H0 in H4.
+    (*inversion X2; subst.
+    inversion X8; subst. *)
+    
+(***)    
+    assert (f0 = FC fenv fps e0 e1 x0 0).
+    eapply (envAppendCompare FunTyping ls0 ls8 ls1 ls3). 
+    eauto.
+    eauto.
+    eauto.
+    auto.
+    auto.
+       
+    rewrite H5 in *.
+  
+    specialize (H1 ftenv).  
+    specialize (H1 0 fenv x0 e0 e1). 
+    specialize (H1 X6 eq_refl).
+    simpl in *.
+    inversion X8; subst.
+
+    assert (t = ret_type).
+    eapply H1. 
+    auto.
+    auto.
+    Focus 2.
+    eauto.
+    auto.
+    rewrite H5.
+    auto.
+    
+  + inversion X; subst.
+    rewrite H0 in H4.
+    (* inversion X2; subst. 
+    inversion X9; subst. *)
+
+    assert (f0 = FC fenv fps e0 e1 x0 (S n0)).
+    eapply (envAppendCompare FunTyping ls0 ls8 ls1 ls3). 
+    eauto.
+    eauto.
+    eauto.
+    auto.
+    auto.
+    
+    rewrite H5 in *.
+
+    specialize (H1 ftenv).  
+    specialize (H1 (S n0) fenv x0 e0 e1). 
+    specialize (H1 X6 eq_refl).
+    simpl in *.
+    inversion X9; subst.
+
+    assert (t = ret_type).
+    eapply H1. 
+    auto.
+    eapply updateFEnvLemma.
+    auto.
+    auto.
+    Focus 2.
+    eauto.
+    subst ftenv'0.
+    eapply updateFEnvLemma.
+    auto.
+    auto.
+    rewrite H5.
+    auto.
+    
+- (* modify *)
+  unfold UniEType.
+  intros ftenv tenv fenv T1 T2 VT1 VT2 XF q K H0 t ftenv0 H0' X.
+  inversion X; subst.
+  eapply inj_pair2 in H6.
+  eapply inj_pair2 in H6; subst.  
+  assert (VT4 = VT1).
+  eapply loc_pi.
+  subst.
+  assert (VT5 = VT2).
+  eapply loc_pi.
+  subst.
+  clear XF2.
+  reflexivity.
+  (* return *)
+- unfold UniEType.
+  intros.
+  inversion X1; subst.
+  inversion X2; subst.
+  inversion k; subst.
+  eapply ValueStrongTyping.
+  eauto.
+  eauto.
+  inversion k; subst.
+  eapply IdStrongTyping.
+  eauto.
+  auto.
+(* bindN *)
+- unfold UniEType.
+  intros.
+  inversion X1; subst.
+  eapply H0.
+  auto.
+  Focus 2.
+  eauto.
+  auto.
+(* bindS *)
+- unfold UniEType.
+  intros.
+  inversion X1; subst.
+  eapply H0.
+  auto.
+  Focus 2.
+  subst tenv'.
+  assert (t1 = t3).
+  eapply H.
+  auto.
+  Focus 2.
+  eauto.
+  auto.
+  rewrite H1.
+  eauto.
+  auto.
+- unfold UniEType.
+  intros.
+  inversion X1; subst.
+  eapply H.
+  eapply overrideEnvLemmaT.
+  assumption.
+  assumption.
+  Focus 2.
+  assert (tenvP = tenvP0).
+  eapply EnvStrongTyping.
+  eauto.
+  auto.
+  rewrite H0.
+  eauto.
+  eapply overrideEnvLemmaT.
+  auto.
+  auto.
+- unfold UniEType, UniQFType, UniPType.
+  intros.  
+  inversion X1; subst.
+  assert (FT fps t = FT fps0 t2).
+  eapply H.
+  auto.
+  eauto.
+  auto.
+  injection H1.
+  auto.
+- unfold UniEType.
+  intros.
+  inversion X1; subst.
+  eapply ValueStrongTyping.
+  eauto.
+  auto.
+- unfold UniEType.
+  intros.
+  inversion X1; subst.
+  eapply H0.
+  auto.
+  Focus 2.
+  eauto.
+  auto.
+- unfold UniEType, Par_SSL, UniPType.
+  intros.
+  dependent induction X; subst.
+  inversion X2; subst.
+  inversion X; subst.
+  auto.
+  destruct pt2.
+  destruct ts.
+  + inversion X2; subst.
+    inversion X3.
+  + inversion m; subst.
+    inversion X2; subst.
+    inversion X5; subst.
+    assert (PT bbs = PT ts).
+    {*  eapply IHX.
+      auto.
+      auto.
+      Focus 2.
+      econstructor.
+      eauto.
+      auto.
+   }   
+   injection H.
+   intro.
+   assert (b = v).
+   {* eapply p0.
+      auto.
+      Focus 2.
+      eauto.
+      auto.
+   }
+   rewrite H0.
+   rewrite H1.
+   auto.
+Qed.   
+   
+
+
+Lemma UniFTypeLm0 (fenv: funEnv) (tenv0: valTC)
+      (e0 e1: Exp) (x: Id) (ft1: FTyp)
+      (k: FunTyping (FC fenv tenv0 e0 e1 x 0) ft1) :
+  UniFType (FC fenv tenv0 e0 e1 x 0) ft1 k ->
+  UniFTypeS (FC fenv tenv0 e0 e1 x 0) ft1 k.
+Proof.
+  unfold UniFTypeS.
+  unfold UniFType, UniFTypeS, UniETypeW.
+  intros.
+  destruct ft1 as [tenv t].
+  destruct ft2.
+  specialize (H tenv t eq_refl).
+  inversion k; subst.
+  inversion X; subst.
+  rename prs_type into tenv.
+  rename ret_type into t0.
+  specialize (H ftenv 0 fenv x e0 e1 X0 eq_refl).
+  simpl in *.
+  specialize (H X1 X0).
+  specialize (H t0 ftenv0 X2 X3).
+  assert (t = t0).
+  eapply ExpStrongTyping.
+  exact X1.
+  auto.
+  exact X2.
+  auto.
+  rewrite H0.
+  auto.
+Qed.
+
+
+Lemma UniFTypeLm0a (fenv: funEnv) (tenv0: valTC)
+      (e0 e1: Exp) (x: Id) (ft1 ft2: FTyp)
+      (k: FunTyping (FC fenv tenv0 e0 e1 x 0) ft1) :
+  UniFType (FC fenv tenv0 e0 e1 x 0) ft1 k ->
+  FunTyping (FC fenv tenv0 e0 e1 x 0) ft2 -> ft1 = ft2.
+  intros.
+  eapply UniFTypeLm0.
+  eauto.
+  auto.
+Qed.
+
+
+Lemma UniFTypeLm0b (fenv: funEnv) (tenv0: valTC)
+      (e0 e1: Exp) (x: Id) (ft1 ft2: FTyp)
+      (k1: FunTyping (FC fenv tenv0 e0 e1 x 0) ft1) 
+      (k2: FunTyping (FC fenv tenv0 e0 e1 x 0) ft2) : ft1 = ft2.
+  intros.
+  inversion k1; subst.
+  inversion k2; subst.
+  assert (t = t0).
+  eapply ExpStrongTyping.
+  exact X0.
+  auto.
+  exact X1.
+  auto.
+  rewrite H.
+  auto.
+Qed.
+
+
+Lemma UniFTypeLm1 (fenv: funEnv) (tenv0: valTC)
+      (e0 e1: Exp) (x: Id) (ft1: FTyp)
+      (k1: FunTyping (FC fenv tenv0 e0 e1 x 1) ft1)
+      (k0: FunTyping (FC fenv tenv0 e0 e1 x 0) ft1):
+  UniFType (FC fenv tenv0 e0 e1 x 1) ft1 k1 ->
+  UniFType (FC fenv tenv0 e0 e1 x 0) ft1 k0.
+Proof.
+  unfold UniFType.
+  intros.
+  destruct ft1 as [tenv1 t1].
+
+  inversion H1; subst.
+  inversion H0; subst.
+  clear H1.
+  clear H0.
+  unfold UniETypeW in *.
+
+  intros.
+  eapply ExpStrongTyping.
+  exact X0.
+  auto.
+  exact X2.
+  auto.
+Qed.
+
+
+Lemma UniFTypeLmN (fenv: funEnv) (tenv0: valTC)
+      (e0 e1: Exp) (x: Id) (n: nat) (ft1: FTyp)
+      (k1: FunTyping (FC fenv tenv0 e0 e1 x (S n)) ft1)
+      (k0: FunTyping (FC fenv tenv0 e0 e1 x n) ft1):
+  UniFType (FC fenv tenv0 e0 e1 x (S n)) ft1 k1 ->
+  UniFType (FC fenv tenv0 e0 e1 x n) ft1 k0.
+Proof.
+  unfold UniFType.
+  intros.
+  destruct ft1 as [tenv1 t1].
+
+  inversion H1; subst.
+  inversion H0; subst.
+  clear H1.
+  clear H0.
+  unfold UniETypeW in *.
+
+  destruct i. 
+  intros.
+  eapply ExpStrongTyping.
+  exact X0.
+  auto.
+  exact X2.
+  auto.
+
+  intros.
+  inversion k0; subst.
+  subst ftenv' fenv'.
+  eapply ExpStrongTyping.
+  exact X5.
+  eapply updateFEnvLemma.
+  auto.
+  auto.
+  eapply X2.
+  auto.
+Qed.
+
+ 
+
+Lemma UniFTypeLm1b (fenv: funEnv) (tenv0: valTC)
+      (e0 e1: Exp) (x: Id) (ft1 ft2: FTyp)
+      (k1: FunTyping (FC fenv tenv0 e0 e1 x 1) ft1) 
+      (k2: FunTyping (FC fenv tenv0 e0 e1 x 0) ft2) : ft1 = ft2.
+  intros.
+  inversion k1; subst.
+  inversion X1; subst.
+  inversion k2; subst.
+  subst ftenv' fenv'. 
+  assert (t = t0).
+  eapply ExpStrongTyping.
+  exact X3.
+  auto.
+  exact X4.
+  auto.
+  rewrite H.
+  auto.
+Qed.
+
+
+
+Lemma UniFTypeLmPb (fenv: funEnv) (tenv0: valTC)
+      (e0 e1: Exp) (x: Id) (n: nat) (ft1 ft2: FTyp)
+      (k1: FunTyping (FC fenv tenv0 e0 e1 x n) ft1) 
+      (k2: FunTyping (FC fenv tenv0 e0 e1 x (S n)) ft2) : ft1 = ft2.
+Proof.
+  intros.
+  inversion k1; subst.
+  
+  - inversion k2; subst.
+    inversion X3; subst.
+    assert (t = t0).
+    {+ eapply ExpStrongTyping.
+       exact X0.
+       auto.
+       exact X4. 
+       auto.
+    }   
+    rewrite H.
+    auto.
+
+  - inversion k2; subst.
+    subst ftenv' fenv' ftenv'0 fenv'0.
+    inversion X4; subst.
+    subst ftenv' fenv'. 
+    assert (t = t0).
+    {+ eapply ExpStrongTyping.
+       exact X0.
+       eapply updateFEnvLemma.
+       auto.
+       auto.
+       eapply updateFEnvLemma.
+       eauto.
+       eauto.
+       auto.
+    }
+    rewrite H.
+    auto.
+Qed.    
+
+Lemma UniFTypeLmNZE1 (fenv: funEnv) (tenv0: valTC)
+      (e0 e1: Exp) (x: Id) (ft: FTyp) :
+  forall n: nat,
+    FunTyping (FC fenv tenv0 e0 e1 x (S n)) ft ->
+    sigT (fun ft0 => FunTyping (FC fenv tenv0 e0 e1 x n) ft0).
+Proof.
+  intros.
+  inversion X; subst.  
+  econstructor.
+  eassumption.
+Qed.
+
+
+
+Lemma UniFTypeLmNZ1 (fenv: funEnv) (tenv0: valTC)
+      (e0 e1: Exp) (x: Id) (ft: FTyp) :
+  forall n: nat,
+    FunTyping (FC fenv tenv0 e0 e1 x (S n)) ft ->
+    FunTyping (FC fenv tenv0 e0 e1 x n) ft.
+Proof.
+  intros.
+  generalize X.
+  eapply UniFTypeLmNZE1 in X.
+  intro.
+  destruct X as [ft0 X].
+  eapply UniFTypeLmPb with (ft1:=ft0) (ft2:=ft) in X0.
+  rewrite <- X0.
+  auto.
+  auto.
+Qed.  
+
+
+Lemma UniFTypeLmNZ (fenv: funEnv) (tenv0: valTC)
+      (e0 e1: Exp) (x: Id) (ft: FTyp) :
+  forall n: nat,
+    FunTyping (FC fenv tenv0 e0 e1 x n) ft ->
+    FunTyping (FC fenv tenv0 e0 e1 x 0) ft.
+Proof.
+  intros.
+  induction n.
+  auto.
+  eapply UniFTypeLmNZ1 in X.
+  eapply IHn.
+  auto.
+Qed.
+
+
+
+Lemma UniFTypeLm (f: Fun) (ft1 ft2: FTyp) (k: FunTyping f ft1) :
+  UniFType f ft1 k ->
+  FunTyping f ft2 -> ft1 = ft2.
+Proof.
+  destruct f.
+  induction n.
+  eapply UniFTypeLm0a.
+  intros.
+  inversion k; subst.
+  eapply (IHn X2).
+  eapply UniFTypeLmN.
+  exact H.
+  inversion X; subst.
+  auto. 
+Qed.  
+
+
+Lemma UniqueFunType (f: Fun) (ft1 ft2: FTyp)
+      (k1: FunTyping f ft1) 
+      (k2: FunTyping f ft2) :  ft1 = ft2.
+Proof.
+  eapply UniFTypeLm with (k:=k1).
+  eapply FunStrongTyping.
+  eauto.
+Qed.
+
+
 End Determ.
